concurrency/lksize.v
@@ -2,6 +2,7 @@ Require Import compcert.common.AST.
 Require Import compcert.common.Memdata.
 Require Import Coq.ZArith.ZArith.
 
-Definition LKCHUNK:= Mint32.
-Definition LKSIZE:= align_chunk LKCHUNK.
+(* LKSIZE should be of the size of the struct we use for locks, which
+happens to be equivalent to an array of 4 pointers, here *)
+Definition LKSIZE:= (4 * 4)%Z.
 Definition LKSIZE_nat:= Z.to_nat LKSIZE.
